positional number system equivalence transcribed from pencil-and-paper proofs by <jadep@mit.edu>

src/Galois/BaseSystem.v
@@ -1,19 +1,18 @@
 Require Import List.
-Require Import ZArith.ZArith.
+Require Import ZArith.ZArith ZArith.Zdiv.
 
 Local Open Scope Z.
-Local Open Scope list_scope.
 
 Module Type BaseCoefs.
   (* lists coefficients of digits and the digits themselves always have the
   * LEAST significant position first. *)
   Definition coefs : Type := list Z.
 
-  Parameter bs : coefs.
+  Parameter base : coefs.
   Axiom bs_good :
     forall i j,
-    let b := nth_default 0 bs in
-    exists r,
+    let b := nth_default 0 base in
+    let r := (b i * b j) / b (i+j)%nat in
     b i * b j = r * b (i+j)%nat.
 End BaseCoefs.
 
@@ -21,7 +20,8 @@ Module BaseSystem (Import B:BaseCoefs).
   Definition digits : Type := list Z.
 
   Definition accumulate p acc := fst p * snd p + acc.
-  Definition decode u  := fold_right accumulate 0 (combine u bs).
+  Definition decode bs u  := fold_right accumulate 0 (combine u bs).
+  Hint Unfold decode accumulate.
 
 	Fixpoint add (us vs:digits) : digits :=
 		match us,vs with
@@ -31,18 +31,198 @@ Module BaseSystem (Import B:BaseCoefs).
 		end.
   Local Infix ".+" := add (at level 50).
 
-  Lemma add_rep : forall us vs, decode (add us vs) = decode us + decode vs.
+  Lemma add_rep : forall bs us vs, decode bs (add us vs) = decode bs us + decode bs vs.
   Proof.
     unfold decode, accumulate.
-    induction bs; destruct us; destruct vs; auto; simpl; try rewrite IHc; ring.
+    induction bs; destruct us; destruct vs; auto; simpl; try rewrite IHbs; ring.
   Qed.
 
-  (* mul' is a valid multiplication algorithm if b_i = b_1^i *)
-  Fixpoint mul' (us vs:digits) : digits :=
+  Lemma decode_nil : forall bs, decode bs nil = 0.
+    auto.
+  Qed.
+
+  (* mul_geomseq is a valid multiplication algorithm if b_i = b_1^i *)
+  Fixpoint mul_geomseq (us vs:digits) : digits :=
 		match us,vs with
-			| u::us', v::vs' => u*v :: map (Z.mul u) vs' .+ mul' us' vs
+			| u::us', v::vs' => u*v :: map (Z.mul u) vs' .+ mul_geomseq us' vs
 			| _, _ => nil
 		end.
 
-  (* UPNEXT: multiplication for arbitrary good bs *)
+  Definition mul_each u := map (Z.mul u).
+  Lemma mul_each_rep : forall bs u vs, decode bs (mul_each u vs) = u * decode bs vs.
+  Proof.
+    unfold decode, accumulate.
+    induction bs; destruct vs; auto; simpl; try rewrite IHbs; ring.
+  Qed.
+
+  Definition crosscoef i j : Z := 
+    let b := nth_default 0 base in
+    (b(i) * b(j)) / b(i+j)%nat.
+
+  Fixpoint zeros n := match n with O => nil | S n' => 0::zeros n' end.
+  Lemma zeros_rep : forall bs n, decode bs (zeros n) = 0.
+    unfold decode, accumulate.
+    induction bs; destruct n; auto; simpl; try rewrite IHbs; ring.
+  Qed.
+  Lemma length_zeros : forall n, length (zeros n) = n.
+    induction n; simpl; auto.
+  Qed.
+
+  Lemma app_zeros_zeros : forall n m, (zeros n ++ zeros m) = zeros (n + m).
+  Admitted.
+
+  Lemma zeros_app0 : forall m, (zeros m ++ 0 :: nil) = zeros (S m).
+  Admitted.
+
+  Lemma rev_zeros : forall n, rev (zeros n) = zeros n.
+  Admitted.
+
+  Lemma app_cons_app_app : forall T xs (y:T) ys, xs ++ y :: ys = (xs ++ (y::nil)) ++ ys.
+  Admitted.
+
+  (* mul' is multiplication with the SECOND ARGUMENT REVERSED and OUTPUT REVERSED *)
+  Fixpoint mul_bi' (i:nat) (vsr:digits) := 
+    match vsr with
+    | v::vsr' => v * crosscoef i (length vsr') :: mul_bi' i vsr'
+    | nil => nil
+    end.
+  Definition mul_bi (i:nat) (vs:digits) : digits :=
+    zeros i ++ rev (mul_bi' i (rev vs)).
+
+  (*
+  Definition mul_bi (i:nat) (vs:digits) : digits :=
+    let mkEntry := (fun (p:(nat*Z)) => let (j, v) := p in v * crosscoef i j) in
+    zeros i ++ map mkEntry (@enumerate Z vs).
+  *)
+
+  Lemma decode_single : forall n bs x,
+    decode bs (zeros n ++ x :: nil) = nth_default 0 bs n * x.
+  Proof.
+    induction n; intros; simpl.
+    destruct bs; auto; unfold decode, accumulate, nth_default; simpl; ring.
+    destruct bs; simpl; auto.
+    unfold decode, accumulate, nth_default in *; simpl in *; auto.
+  Qed.
+
+  Lemma peel_decode : forall xs ys x y, decode (x::xs) (y::ys) = x*y + decode xs ys.
+    intros.
+    unfold decode, accumulate, nth_default in *; simpl in *; ring_simplify; auto.
+  Qed.
+
+  Lemma decode_highzeros : forall xs bs n, decode bs (xs ++ zeros n) = decode bs xs.
+    induction xs; intros; simpl; try rewrite zeros_rep; auto.
+    destruct bs; simpl; auto.
+    repeat (rewrite peel_decode).
+    rewrite IHxs; auto.
+  Qed.
+
+  Lemma mul_bi_single : forall m n x,
+    decode base (mul_bi n (zeros m ++ x :: nil)) = nth_default 0 base m * x * nth_default 0 base n.
+  Proof.
+    unfold mul_bi.
+    destruct m; simpl; ssimpl_list; simpl; intros.
+    rewrite decode_single.
+    unfold crosscoef; simpl.
+    rewrite plus_0_r.
+    ring_simplify.
+    replace (nth_default 0 base n * nth_default 0 base 0) with (nth_default 0 base 0 * nth_default 0 base n) by ring.
+    SearchAbout Z.div.
+    rewrite Z_div_mult; try ring.
+
+    assert (nth_default 0 base n > 0) by admit; auto.
+
+    intros; simpl; ssimpl_list; simpl.
+    replace (mul_bi' n (rev (zeros m) ++ 0 :: nil)) with (zeros (S m)) by admit.
+    intros; simpl; ssimpl_list; simpl.
+    rewrite length_zeros.
+    rewrite app_cons_app_app.
+    rewrite rev_zeros.
+    intros; simpl; ssimpl_list; simpl.
+    rewrite zeros_app0.
+    rewrite app_assoc.
+    rewrite app_zeros_zeros.
+    rewrite decode_single.
+    unfold crosscoef; simpl; ring_simplify.
+    rewrite NPeano.Nat.add_1_r.
+    rewrite bs_good.
+    rewrite Z_div_mult.
+    rewrite <- Z.mul_assoc.
+    rewrite <- Z.mul_comm.
+    rewrite <- Z.mul_assoc.
+    rewrite <- Z.mul_assoc.
+    destruct (Z.eq_dec x 0); subst; try ring.
+    rewrite Z.mul_cancel_l by auto.
+    rewrite <- bs_good.
+    ring.
+
+    assert (nth_default 0 base (n + S m) > 0) by admit; auto.
+  Qed.
+
+  Lemma set_higher' : forall vs x, vs++x::nil = vs .+ (zeros (length vs) ++ x :: nil).
+    induction vs; auto.
+    intros; simpl; rewrite IHvs; f_equal; ring.
+  Qed.
+  
+  Lemma set_higher : forall bs vs x,
+    decode bs (vs++x::nil) = decode bs vs + nth_default 0 bs (length vs) * x.
+  Proof.
+    intros.
+    rewrite set_higher'.
+    rewrite add_rep.
+    f_equal.
+    apply decode_single.
+  Qed.
+
+  Lemma zeros_plus_zeros : forall n, zeros n = zeros n .+ zeros n.
+    induction n; auto.
+    simpl; f_equal; auto. 
+  Qed.
+
+  Lemma mul_bi_add : forall n us vs,
+    mul_bi n (us .+ vs) = mul_bi n us .+ mul_bi n vs.
+  Proof.
+  Admitted.
+
+  Lemma mul_bi_rep : forall i vs, decode base (mul_bi i vs) = decode base vs * nth_default 0 base i.
+    induction vs using rev_ind; intros; simpl. {
+      unfold mul_bi.
+      ssimpl_list; rewrite zeros_rep; simpl.
+      unfold decode; simpl.
+      ring.
+    } {
+      rewrite set_higher.
+      ring_simplify.
+      rewrite <- IHvs; clear IHvs.
+      rewrite <- mul_bi_single.
+      rewrite <- add_rep.
+      rewrite <- mul_bi_add.
+      rewrite set_higher'.
+      auto.
+    }
+  Qed.
+
+  (* mul' is multiplication with the FIRST ARGUMENT REVERSED *)
+  Fixpoint mul' (usr vs:digits) : digits :=
+		match usr with
+			| u::usr' => 
+            mul_each u (mul_bi (length usr') vs) .+ mul' usr' vs
+			| _ => nil
+    end.
+  Definition mul us := mul' (rev us).
+  Local Infix "#*" := mul (at level 40).
+
+  Lemma mul'_rep : forall us vs, decode base (mul' (rev us) vs) = decode base us * decode base vs.
+    induction us using rev_ind; intros; simpl; try apply decode_nil.
+    ssimpl_list.
+    rewrite add_rep.
+    rewrite IHus; clear IHus.
+    rewrite set_higher.
+    rewrite mul_each_rep.
+    rewrite mul_bi_rep.
+    ring.
+  Qed.
+
+  Lemma mul_rep : forall us vs, decode base (us #* vs) = decode base us * decode base vs.
+    apply mul'_rep.
+  Qed.
 End BaseSystem.
